@prefix : <https://www.bim-sis.de/ontology/sco#> .
@prefix bot: <https://w3id.org/bot#> .
@prefix owl: <http://www.w3.org/2002/07/owl#> .
@prefix rdf: <http://www.w3.org/1999/02/22-rdf-syntax-ns#> .
@prefix sco: <https://www.bim-sis.de/ontology/sco#> .
@prefix xml: <http://www.w3.org/XML/1998/namespace> .
@prefix xsd: <http://www.w3.org/2001/XMLSchema#> .
@prefix foaf: <http://xmlns.com/foaf/0.1/> .
@prefix rdfs: <http://www.w3.org/2000/01/rdf-schema#> .
@prefix vann: <http://purl.org/vocab/vann/> .
@prefix dcterms: <http://purl.org/dc/terms> .
@base <https://www.bim-sis.de/ontology/sco#> .

<https://www.bim-sis.de/ontology/sco#> rdf:type owl:Ontology ;
                                        owl:versionIRI <https://www.bim-sis.de/ontology/sco#/0.1.0> ;
                                        dcterms:creator [ rdf:type foaf:Person ;
                                                          foaf:name "Al-Hakam Hamdan"
                                                        ] ,
                                                        [ rdf:type foaf:Person ;
                                                          foaf:name "Mushtak Seeaed"
                                                        ] ;
                                        dcterms:description "Ontology for describing stone components in masonry structures"@en ;
                                        dcterms:license "https://creativecommons.org/licenses/by/1.0" ;
                                        dcterms:modified "June 28st 2021" ;
                                        dcterms:title "Stone Component Ontology"@en ;
                                        vann:preferredNamespacePrefix "sco" ;
                                        vann:preferredNamespaceUri "https://www.bim-sis.de/ontology/sco#" .

#################################################################
#    Object Properties
#################################################################

###  https://www.bim-sis.de/ontology/sco#adjacentJoint
sco:adjacentJoint rdf:type owl:ObjectProperty ;
                  rdfs:subPropertyOf sco:adjacentStoneComponent ;
                  rdfs:domain sco:StoneComponent ;
                  rdfs:range sco:Joint ;
                  rdfs:comment "Describes the relationship between a stone component (either stone or joint) and an adjacent joint."@en ;
                  rdfs:label "adjacent joint"@en .


###  https://www.bim-sis.de/ontology/sco#adjacentStone
sco:adjacentStone rdf:type owl:ObjectProperty ;
                  rdfs:subPropertyOf sco:adjacentStoneComponent ;
                  rdfs:domain sco:StoneComponent ;
                  rdfs:range sco:Stone ;
                  rdfs:comment "Describes the relationship between a stone component (either stone or joint) and an adjacent stone."@en ;
                  rdfs:label "adjacent stone"@en .


###  https://www.bim-sis.de/ontology/sco#adjacentStoneComponent
sco:adjacentStoneComponent rdf:type owl:ObjectProperty ;
                           rdfs:domain sco:StoneComponent ;
                           rdfs:range sco:StoneComponent ;
                           rdfs:comment "Describes the relationship between two adjacent Stone Component individuals."@en ;
                           rdfs:label "adjacent stone component"@en .


###  https://www.bim-sis.de/ontology/sco#aggregatesJoint
sco:aggregatesJoint rdf:type owl:ObjectProperty ;
                    rdfs:subPropertyOf sco:aggregatesStoneComponent ;
                    rdfs:domain bot:Element ;
                    rdfs:range sco:Joint ;
                    rdfs:comment "Describes the relationship between a building element (e.g. a wall) and a joint that is aggregated as part of the element."@en ;
                    rdfs:label "aggregates joint"@en .


###  https://www.bim-sis.de/ontology/sco#aggregatesStone
sco:aggregatesStone rdf:type owl:ObjectProperty ;
                    rdfs:subPropertyOf sco:aggregatesStoneComponent ;
                    rdfs:domain bot:Element ;
                    rdfs:range sco:Stone ;
                    rdfs:comment "Describes the relationship between a building element (e.g. a wall) and a stone that is aggregated as part of the element."@en ;
                    rdfs:label "aggregates stone"@en .


###  https://www.bim-sis.de/ontology/sco#aggregatesStoneComponent
sco:aggregatesStoneComponent rdf:type owl:ObjectProperty ;
                             rdfs:subPropertyOf bot:hasSubElement ;
                             rdfs:domain bot:Element ;
                             rdfs:range sco:StoneComponent ;
                             rdfs:comment "Describes the relationship between a building element (e.g. a wall) and a stone component that is aggregated as part of the element."@en ;
                             rdfs:label "aggregates stone component"@en .


#################################################################
#    Data properties
#################################################################

###  https://www.bim-sis.de/ontology/sco#jointDimensional
sco:jointDimensional rdf:type owl:DatatypeProperty ;
                     rdfs:domain sco:Joint ;
                     rdfs:comment "Defines a size specification of a joint, such as width or depth."@en ;
                     rdfs:label "joint dimensional"@en .


###  https://www.bim-sis.de/ontology/sco#jointWidth
sco:jointWidth rdf:type owl:DatatypeProperty ;
               rdfs:subPropertyOf sco:jointDimensional ;
               rdfs:domain sco:Joint ;
               rdfs:comment "Defines the width of a joint. Unit in [mm]."@en ;
               rdfs:label "joint width"@en .


###  https://www.bim-sis.de/ontology/sco#stoneDimensional
sco:stoneDimensional rdf:type owl:DatatypeProperty ;
                     rdfs:domain sco:Stone ;
                     rdfs:comment "Defines a size specification of a stone, such as width or depth."@en ;
                     rdfs:label "stone dimensional"@en .


###  https://www.bim-sis.de/ontology/sco#stoneHeight
sco:stoneHeight rdf:type owl:DatatypeProperty ;
                rdfs:subPropertyOf sco:stoneDimensional ;
                rdfs:domain sco:Stone ;
                rdfs:comment "Defines the height of a stone. Unit in [cm]."@en ;
                rdfs:label "stone height"@en .


###  https://www.bim-sis.de/ontology/sco#stoneLength
sco:stoneLength rdf:type owl:DatatypeProperty ;
                rdfs:subPropertyOf sco:stoneDimensional ;
                rdfs:domain sco:Stone ;
                rdfs:comment "Defines the length of a stone. Unit in [cm]."@en ;
                rdfs:label "stone length"@en .


###  https://www.bim-sis.de/ontology/sco#stoneWidth
sco:stoneWidth rdf:type owl:DatatypeProperty ;
               rdfs:subPropertyOf sco:stoneDimensional ;
               rdfs:domain sco:Stone ;
               rdfs:comment "Defines the width of a stone. Unit in [cm]."@en ;
               rdfs:label "stone width"@en .


#################################################################
#    Classes
#################################################################


###  https://www.bim-sis.de/ontology/sco#Joint
sco:Joint rdf:type owl:Class ;
          rdfs:subClassOf sco:StoneComponent ;
          rdfs:comment "Describes the area between adjacent stones. Is usually mortared."@en ;
          rdfs:label "Joint"@en .


###  https://www.bim-sis.de/ontology/sco#Stone
sco:Stone rdf:type owl:Class ;
          rdfs:subClassOf sco:StoneComponent ;
          rdfs:comment "A stone is a compact object made of minerals or rock, which could be used for buliding bearing structures."@en ;
          rdfs:label "Stone"@en .


###  https://www.bim-sis.de/ontology/sco#StoneComponent
sco:StoneComponent rdf:type owl:Class ;
                   rdfs:subClassOf bot:Element ;
                   rdfs:comment "Component of a masonry structure, usually a stone or mortared joint."@en ;
                   rdfs:label "Stone component"@en .


[ rdf:type foaf:Person ;
  foaf:name "Al-Hakam Hamdan"
] .

[ rdf:type foaf:Person ;
   foaf:name "Mushtak Seeaed"
 ] .
