@prefix cdo: <https://wisib.de/ontologie/damage/cdo#> .
@prefix dot: <https://w3id.org/dot#> .
@prefix dce: <http://purl.org/dc/elements/1.1/> .
@prefix owl: <http://www.w3.org/2002/07/owl#> .
@prefix rdf: <http://www.w3.org/1999/02/22-rdf-syntax-ns#> .
@prefix xml: <http://www.w3.org/XML/1998/namespace> .
@prefix xsd: <http://www.w3.org/2001/XMLSchema#> .
@prefix foaf: <http://xmlns.com/foaf/0.1/> .
@prefix rdfs: <http://www.w3.org/2000/01/rdf-schema#> .
@prefix vann: <http://purl.org/vocab/vann/> .
@prefix props: <https://w3id.org/product/props#> .
@prefix dcterms: <http://purl.org/dc/terms> .

<https://wisib.de/ontologie/damage/cdo#> rdf:type owl:Ontology ;
                         owl:versionIRI <https://wisib.de/ontologie/damage/cdo#/0.5.0> ;
                         dcterms:creator [ rdf:type foaf:Person ;
                                           foaf:name "Al-Hakam Hamdan"
                                         ] ,
                                         [ foaf:name "Mathias Bonduel" ;
                                           rdf:type foaf:Person
                                         ] ;
                         dcterms:description "Ontology for damage and defects in reinforced concrete."@en ;
                         dcterms:license "https://creativecommons.org/licenses/by/1.0" ;
                         dcterms:modified "September 16th 2020" ;
                         dcterms:title "Concrete Damage Ontology"@en ;
                         vann:preferredNamespacePrefix "cdo" ;
                         vann:preferredNamespaceUri "https://wisib.de/ontologie/damage/cdo#" .


#################################################################
#    Data properties
#################################################################

###  https://wisib.de/ontologie/damage/cdo#crackAngle
cdo:crackAngle rdf:type owl:DatatypeProperty ;
               rdfs:domain cdo:Crack ;
               rdfs:comment """Defines the angle of the crack in relation to local coordinate system of the damaged component.

Unit in [°]."""@en ;
               rdfs:label "crack angle"@en .


###  https://wisib.de/ontologie/damage/cdo#crackDepth
cdo:crackDepth rdf:type owl:DatatypeProperty ;
               rdfs:subPropertyOf props:depth ;
               rdfs:domain cdo:Crack ;
               rdfs:comment "Unit in [mm]."@en ;
               rdfs:label "crack depth"@en .


###  https://wisib.de/ontologie/damage/cdo#crackSpacing
cdo:crackSpacing rdf:type owl:DatatypeProperty ;
                 rdfs:domain cdo:Crack ;
                 rdfs:comment "Defines the crack spacing."@en ;
                 rdfs:label "crackSpacing" .


###  https://wisib.de/ontologie/damage/cdo#crackWidth
cdo:crackWidth rdf:type owl:DatatypeProperty ;
               rdfs:subPropertyOf props:width ;
               rdfs:domain cdo:Crack ;
               rdfs:comment "Defines the crack width. Unit: mm"@en ;
               rdfs:label "crack width" .


###  https://wisib.de/ontologie/damage/cdo#spallingArea
cdo:spallingArea rdf:type owl:DatatypeProperty ;
                 rdfs:domain cdo:Spalling ;
                 rdfs:comment "Defines the area value of a spalling. Unit in mm²."@en ;
                 rdfs:label "spalling area" .


#################################################################
#    Classes
#################################################################


###  https://wisib.de/ontologie/damage/cdo#AutogenousShrinkageCrack
cdo:ConcreteDamage rdf:type owl:Class ;
                   rdfs:subClassOf dot:ClassifiedDamage ;
                   rdfs:comment "A classified damage that appears on building elements made of concrete"@en ;
                         rdfs:label "Betonschaden"@de ,
                                    "Concrete Damage"@en .

###  https://wisib.de/ontologie/damage/cdo#AlkaliSilicaReaction
cdo:AlkaliSilicaReaction rdf:type owl:Class ;
                         rdfs:subClassOf cdo:Efflorescence ,
                                         cdo:ReticulatedCrackArea ,
                                         dot:StructuralDamage ;
                         rdfs:comment """Swelling reaction that occurs over time in concrete between the highly alkaline cement paste and the reactive non-crystalline (amorphous) silica found in many common aggregates, given sufficient moisture.

This reaction causes the expansion of the altered aggregate by the formation of a soluble and viscous gel of sodium silicate (Na2SiO3 • nH2O, also noted Na2H2SiO4 • nH2O, or N-S-H (sodium silicate hydrate), depending the adopted convention). This hygroscopic gel swells and increases in volume when absorbing water: it exerts an expansive pressure inside the siliceous aggregate, causing spalling and loss of strength of the concrete, finally leading to its failure.

ASR can lead to serious cracking in concrete, resulting in critical structural problems that can even force the demolition of a particular structure."""@en ;
                         rdfs:label "Alkali-Kieselsäure-Reaktion"@de ,
                                    "Alkali-silica reaction"@en .


###  https://wisib.de/ontologie/damage/cdo#AutogenousShrinkageCrack
cdo:AutogenousShrinkageCrack rdf:type owl:Class ;
                             rdfs:subClassOf cdo:ShrinkageCrack .


###  https://wisib.de/ontologie/damage/cdo#BendingCrack
cdo:BendingCrack rdf:type owl:Class ;
                 rdfs:subClassOf cdo:Crack ;
                 rdfs:label "Bending Crack"@en ,
                            "Biegeriss"@de .


###  https://wisib.de/ontologie/damage/cdo#Carbonatation
cdo:Carbonatation rdf:type owl:Class ;
                  rdfs:subClassOf cdo:ChemicalDamage ;
                  rdfs:comment "Carbonatation leads to a decrease of the alkalinity, which is essential for corrosion prevention of the reinforcement steel."@en ;
                  rdfs:label "Carbonatation"@en .


###  https://wisib.de/ontologie/damage/cdo#Cavity
cdo:Cavity rdf:type owl:Class ;
           rdfs:subClassOf cdo:ConcreteInhomogeneity ;
           rdfs:comment "Defines an area or spot of cavities."@en ;
           rdfs:label "Cavity"@en ,
                      "Hohlstelle"@de .


###  https://wisib.de/ontologie/damage/cdo#ChemicalDamage
cdo:ChemicalDamage rdf:type owl:Class ;
                   rdfs:subClassOf cdo:ConcreteDamage ;
                   rdfs:comment "Damage that is caused by chemical reactions in the concrete material or the reinforcement."@en ;
                   rdfs:label "Chemical Damage"@en .


###  https://wisib.de/ontologie/damage/cdo#ChlorideAttack
cdo:ChlorideAttack rdf:type owl:Class ;
                   rdfs:subClassOf cdo:ChemicalDamage ;
                   rdfs:comment "Calcium chloride and (to a lesser extent) sodium chloride have been shown to leach calcium hydroxide and cause chemical changes in Portland cement, leading to loss of strength, as well as attacking the steel reinforcement present in most concrete."@en ;
                   rdfs:label "Chloride Attack"@en .


###  https://wisib.de/ontologie/damage/cdo#CoarseGrainAggregate
cdo:CoarseGrainAggregate rdf:type owl:Class ;
                         rdfs:subClassOf cdo:ConcreteInhomogeneity ;
                         rdfs:comment "Area of coarse grain inside the concrete structure"@en ;
                         rdfs:label "Coarse Grain Aggregate"@en ,
                                    "Grobkornstelle"@de .


###  https://wisib.de/ontologie/damage/cdo#ConcreteInhomogeneity
cdo:ConcreteInhomogeneity rdf:type owl:Class ;
                          rdfs:subClassOf cdo:ConcreteDamage ;
                          rdfs:comment "Describes inhomogeneities inside the concrete structure."@en ;
                          rdfs:label "Concrete Inhomogeneity"@en .


###  https://wisib.de/ontologie/damage/cdo#Crack
cdo:Crack rdf:type owl:Class ;
          rdfs:subClassOf cdo:ConcreteDamage ;
          rdfs:comment "A defect that defines a discontinuity in the structure due to material failuer / exceeding the breaking strength of the material."@en ;
          rdfs:label "Crack"@en .


###  https://wisib.de/ontologie/damage/cdo#DiagonalCrack
cdo:DiagonalCrack rdf:type owl:Class ;
                  rdfs:subClassOf cdo:Crack ,
                                  cdo:LongitudinalCrack ,
                                  cdo:TransverseCrack ;
                  rdfs:comment "Caused by shearing"@en ;
                  rdfs:label "Diagonal Crack"@en .


###  https://wisib.de/ontologie/damage/cdo#Efflorescence
cdo:Efflorescence rdf:type owl:Class ;
                  rdfs:subClassOf cdo:MoistureDamage ;
                  rdfs:comment "Efflorescences are white, veil-like to stained coverings on concrete surfaces. They can change colour, especially when dry, and thus impair the appearance and appearance of visible concrete surfaces. Efflorescence has no influence on the strength and durability and thus on the properties of the concrete."@en ;
                  rdfs:label "Ausblühungen"@de ,
                             "Efflorescence"@en .


###  https://wisib.de/ontologie/damage/cdo#HydrationHeatCrack
cdo:HydrationHeatCrack rdf:type owl:Class ;
                       rdfs:subClassOf cdo:Crack ;
                       rdfs:comment "Riss aufgrund von Hydratationswärme (Eigenspannungen vorhanden)"@de ;
                       rdfs:label "Hydratationswärme-Riss"@de .


###  https://wisib.de/ontologie/damage/cdo#ImpurityConfinement
cdo:ImpurityConfinement rdf:type owl:Class ;
                        rdfs:subClassOf cdo:ConcreteInhomogeneity ;
                        rdfs:comment "Defines an area or spot where an object or impurity is confined inside the concrete."@en ;
                        rdfs:label "Fremdkörpereinschluss"@de ,
                                   "Impurity Confinement"@en .


###  https://wisib.de/ontologie/damage/cdo#LongitudinalCrack
cdo:LongitudinalCrack rdf:type owl:Class ;
                      rdfs:subClassOf cdo:Crack ;
                      rdfs:label "Longitudinal Crack"@en .


###  https://wisib.de/ontologie/damage/cdo#MoistureDamage
cdo:MoistureDamage rdf:type owl:Class ;
                   rdfs:subClassOf cdo:ConcreteDamage ;
                   rdfs:comment "Moisture damage is defined as direct and indirect structural damage caused to a building or structure by moisture. This can either be the result of external weather influences, soil moisture or condensation."@en ;
                   rdfs:label "Moisture Damage"@en .


###  https://wisib.de/ontologie/damage/cdo#MoisturePenetration
cdo:MoisturePenetration rdf:type owl:Class ;
                        rdfs:subClassOf cdo:MoistureDamage ;
                        rdfs:comment "Defines a (partially) moisture penetration."@en ;
                        rdfs:label "(stellenweise) Durchfeuchtung"@de ,
                                   "Moisture Penetration"@en .


###  https://wisib.de/ontologie/damage/cdo#PlasticShrinkageCrack
cdo:PlasticShrinkageCrack rdf:type owl:Class ;
                          rdfs:subClassOf cdo:ShrinkageCrack .


###  https://wisib.de/ontologie/damage/cdo#ReinforcementCorrosion
cdo:ReinforcementCorrosion rdf:type owl:Class ;
                           rdfs:subClassOf cdo:ChlorideAttack ,
                                           cdo:ReinforcementDamage ;
                           rdfs:comment "Chloride Damage, where reinforcement has been corroded. The brown outline of the corroded reinforcement can be seen at the surface of the concrete."@en ;
                           rdfs:label "Reinforcement Corrosion"@en .


###  https://wisib.de/ontologie/damage/cdo#ReinforcementCorrosionCrossSectionReduction
cdo:ReinforcementCorrosionCrossSectionReduction rdf:type owl:Class ;
                                                rdfs:subClassOf cdo:ReinforcementCorrosion ;
                                                rdfs:comment "Defines a reinforcement corrosion where the cross section of the reinforcing bars is visibly reduced."@en ;
                                                rdfs:label "Reinforcement Corrosion with cross-section reduction"@en ,
                                                           "korrodierte Tragbewehrung mit Querschnittsminderung"@de .


###  https://wisib.de/ontologie/damage/cdo#ReinforcementDamage
cdo:ReinforcementDamage rdf:type owl:Class ;
                        rdfs:subClassOf cdo:ConcreteDamage ;
                        rdfs:comment "Defines a damage that affects the reinforcement inside a concrete component"@en ;
                        rdfs:label "Bewehrungsschaden"@de ,
                                   "Reinforcement Damage"@en .


###  https://wisib.de/ontologie/damage/cdo#ReticulatedCrackArea
cdo:ReticulatedCrackArea rdf:type owl:Class ;
                         rdfs:subClassOf cdo:Crack ,
                                         dot:DamageArea ;
                         rdfs:label "Reticulated Crack Area"@en .


###  https://wisib.de/ontologie/damage/cdo#RustStaining
cdo:RustStaining rdf:type owl:Class ;
                 rdfs:subClassOf cdo:Efflorescence ;
                 rdfs:comment "Efflorescence of ferrous aggregates."@en ;
                 rdfs:label "Ausblühung eisenhaltiger Zuschlagstoffe / Rostfahne"@de ,
                            "Rust Staining"@en .


###  https://wisib.de/ontologie/damage/cdo#SettlementCrack
cdo:SettlementCrack rdf:type owl:Class ;
                    rdfs:subClassOf cdo:ShrinkageCrack .


###  https://wisib.de/ontologie/damage/cdo#ShrinkageCrack
cdo:ShrinkageCrack rdf:type owl:Class ;
                   rdfs:subClassOf cdo:Crack ;
                   rdfs:label "Shrinkage Crack"@en .


###  https://wisib.de/ontologie/damage/cdo#Sintering
cdo:Sintering rdf:type owl:Class ;
              rdfs:subClassOf cdo:MoistureDamage ,
                              dot:Defect ;
              rdfs:comment """If water seeps through a concrete body, it absorbs soluble components on its way out of the cement, sometimes also from the aggregate. If this water then comes to the surface and evaporates, the components dissolved in it remain behind and form stains.

Internal sintering can be traced back to defects in the execution, to leaking concrete, to improper construction joints and to destruction inside a concrete component."""@en ;
              rdfs:label "Aussintern"@de ,
                         "Sintering"@en .


###  https://wisib.de/ontologie/damage/cdo#Spalling
cdo:Spalling rdf:type owl:Class ;
             rdfs:subClassOf cdo:ConcreteDamage ;
             rdfs:comment "A defect where the concrete is slowly broken down into small flakes known as spalls from a larger solidified concrete body."@en ;
             rdfs:label "Spalling"@en .


###  https://wisib.de/ontologie/damage/cdo#SpallingExposedReinforcement
cdo:SpallingExposedReinforcement rdf:type owl:Class ;
                                 rdfs:subClassOf cdo:ReinforcementDamage ,
                                                 cdo:Spalling ;
                                 rdfs:comment "A spalling where the reinforcement is exposed."@en ;
                                 rdfs:label "Abplatzung mit freiliegender Bewehrung"@de ,
                                            "Spalling with exposed Reinforcement"@en .


###  https://wisib.de/ontologie/damage/cdo#SplittingCrack
cdo:SplittingCrack rdf:type owl:Class ;
                   rdfs:subClassOf cdo:Crack ,
                                   dot:StructuralDamage ;
                   rdfs:comment "Cracks that run through the cross-section of the entire structure / component."@en ;
                   rdfs:label "Splitting Crack"@en ,
                              "Trennriss"@de .


###  https://wisib.de/ontologie/damage/cdo#StressCorrosionCrack
cdo:StressCorrosionCrack rdf:type owl:Class ;
                         rdfs:subClassOf cdo:TendonDamage ;
                         rdfs:comment "Stress corrosion cracking (SCC) is the growth of crack formation in a corrosive environment. It can lead to unexpected sudden failure of normally ductile metal alloys subjected to a tensile stress, especially at elevated temperature."@en ;
                         rdfs:label "Spannungsrisskorrosion"@de ,
                                    "Stress Corrosion Crack"@en .


###  https://wisib.de/ontologie/damage/cdo#StressCorrosionCrack
cdo:TendonCorrosion rdf:type owl:Class ;
                         rdfs:subClassOf cdo:TendonDamage ;
                         rdfs:comment "Corrosion that affects the tendon or a part of it"@en ;
                         rdfs:label "Spannstahlkorrosion"@de ,
                                    "Tendon Corrosion"@en .


###  https://wisib.de/ontologie/damage/cdo#SulfateAttack
cdo:SulfateAttack rdf:type owl:Class ;
                  rdfs:subClassOf cdo:ChemicalDamage ;
                  rdfs:comment "Sulfates in solution in contact with concrete can cause chemical changes to the cement, which can cause significant microstructural effects leading to the weakening of the cement binder (chemical sulfate attack)."@en ;
                  rdfs:label "Sulfate Attack"@en .


###  https://wisib.de/ontologie/damage/cdo#SurfaceCrack
cdo:SurfaceCrack rdf:type owl:Class ;
                 rdfs:subClassOf cdo:Crack ;
                 rdfs:label "Surface Crack"@en .


###  https://wisib.de/ontologie/damage/cdo#TendonDamage
cdo:TendonDamage rdf:type owl:Class ;
                 rdfs:subClassOf cdo:ConcreteDamage ;
                 rdfs:comment "Defines a damage that affects the Tendon inside a concrete structure"@en ;
                 rdfs:label "Spannstahlschaden"@de ,
                            "Tendon Damage"@en .


###  https://wisib.de/ontologie/damage/cdo#TendonParallelCrack
cdo:TendonParallelCrack rdf:type owl:Class ;
                        rdfs:subClassOf cdo:Crack ;
                        rdfs:comment "Crack that is parallel to the aggregated tendon (in general Transverse Crack)."@en ;
                        rdfs:label "Spannstahlparalleler Riss"@de ,
                                   "Tendon parallel crack"@en .


###  https://wisib.de/ontologie/damage/cdo#TransverseCrack
cdo:TransverseCrack rdf:type owl:Class ;
                    rdfs:subClassOf cdo:Crack ;
                    rdfs:label "Transverse Crack"@en .
